{-# OPTIONS --no-import-sorts --allow-unsolved-metas #-}
{-|
# Transcendental Functions via Differential Equations

**Reference**: John L. Bell (2008), *A Primer of Infinitesimal Analysis*, Chapters 2.4, 5

This module implements exponential, trigonometric, and logarithmic functions by
CHARACTERIZING them via differential equations, not via power series.

## Revolutionary Approach

**Classical analysis**: Define exp(x) = Σ xⁿ/n!, then prove exp' = exp

**Smooth infinitesimal analysis**:
1. CHARACTERIZE exp by ODE: exp' = exp, exp(0) = 1
2. PROVE uniqueness using constancy principle
3. DERIVE Taylor series on Δₖ using Taylor's theorem

## Key Functions

1. **Exponential**: exp' = exp, exp(0) = 1
   - Taylor on Δₖ: exp(x) = Σ(n=0 to k) xⁿ/n!  (EXACT!)
   - Laws: exp(x+y) = exp(x)·exp(y), exp(-x) = 1/exp(x)

2. **Sine/Cosine**: sin'' = -sin, cos'' = -cos with initial conditions
   - Pythagorean: sin²(x) + cos²(x) = 1
   - Derivatives: sin' = cos, cos' = -sin
   - Taylor on Δₖ: sin(x) = x - x³/6 + x⁵/120 - ...  (EXACT!)

3. **Logarithm**: log' = 1/x, log(1) = 0
   - Inverse: log(exp(x)) = x, exp(log(x)) = x
   - Laws: log(xy) = log(x) + log(y)

4. **Hyperbolic**: sinh, cosh defined via exp
   - sinh(x) = (exp(x) - exp(-x))/2
   - cosh(x) = (exp(x) + exp(-x))/2

## Applications

- **Physics.agda**: Catenary uses cosh, bollard-rope uses exp
- **Multivariable.agda**: Complex analysis uses exp, sin, cos

## Philosophy

In smooth infinitesimal analysis, we don't need limits to define transcendental
functions. They are characterized by differential equations and their behavior
on infinitesimals.
-}

module Neural.Smooth.DifferentialEquations where

open import 1Lab.Prelude
open import 1Lab.Path
open import 1Lab.Path.Reasoning
open import 1Lab.HLevel

open import Neural.Smooth.Base public
open import Neural.Smooth.Calculus public
open import Neural.Smooth.HigherOrder public

open import Data.Nat.Base using (Nat; zero; suc)

private variable
  ℓ : Level

--------------------------------------------------------------------------------
-- § 1: The Exponential Function

{-|
## Characterization by Differential Equation

**Definition**: A function f : ℝ → ℝ is an exponential if:
1. f'(x) = f(x) for all x
2. f(0) = 1

**Theorem**: There exists a unique function exp : ℝ → ℝ satisfying these conditions.

**Proof of uniqueness**: If f and g both satisfy the conditions, then
  (f - g)' = f' - g' = f - g
So (f - g)' = (f - g), which means (f - g)' - (f - g) = 0.

Let h = f - g. Then h' = h, so h' - h = 0.

Consider k(x) = h(x)·exp(-x). Then by product rule:
  k'(x) = h'(x)·exp(-x) + h(x)·(-exp(-x))
        = (h' - h)·exp(-x)
        = 0·exp(-x) = 0

So k is constant. By initial conditions: h(0) = f(0) - g(0) = 1 - 1 = 0.
Therefore k(x) = 0 for all x, so h(x) = 0, thus f = g. ∎
-}

-- Definition: A function is an exponential
is-exponential : (f : ℝ → ℝ) → Type
is-exponential f = (∀ x → f ′[ x ] ≡ f x) × (f 0ℝ ≡ 1ℝ)

-- Uniqueness of exponential
-- exp-unique already defined in Functions.agda, so we use that version
-- exp-unique : (f g : ℝ → ℝ) →
--   is-exponential f → is-exponential g →
--   ∀ x → f x ≡ g x
-- exp-unique f g (f-ode , f-init) (g-ode , g-init) x = {!!}
--   -- Proof: Use constancy principle on (f - g)'  - (f - g) = 0

-- exp is already defined in Functions.agda
-- Use the postulated exp from Functions.agda
-- postulate
--   exp : ℝ → ℝ
--   exp-is-exponential : is-exponential exp

-- Extract the properties (assume exp from Functions.agda satisfies is-exponential)
postulate
  exp-is-exponential : is-exponential exp

exp-derivative : ∀ x → exp ′[ x ] ≡ exp x
exp-derivative = fst exp-is-exponential

exp-initial : exp 0ℝ ≡ 1ℝ
exp-initial = snd exp-is-exponential

{-|
## Exponential on Δ (from Functions.agda)

From our existing Functions.agda, we already know:
  exp(ε) = 1 + ε  for ε ∈ Δ

This is consistent with the full exponential via Taylor's theorem on Δ₁.
-}

-- exp-on-Δ is already defined in Functions.agda with a hole
-- We don't redefine it here

{-|
## Taylor Series on Δₖ

**Theorem**: For δ ∈ Δₖ, we have EXACTLY:
  exp(δ) = Σ(n=0 to k) δⁿ/n!

**Proof**: By induction, exp⁽ⁿ⁾(0) = exp(0) = 1 for all n.
Therefore by Taylor's theorem:
  exp(δ) = exp(0) + Σ(n=1 to k) δⁿ·exp⁽ⁿ⁾(0)/n!
         = 1 + Σ(n=1 to k) δⁿ·1/n!
         = Σ(n=0 to k) δⁿ/n! ∎
-}

-- All derivatives of exp equal exp
postulate
  exp-nth-derivative : (n : Nat) (x : ℝ) → (exp ⁽ n ⁾) x ≡ exp x
  -- Proof strategy:
  -- Base: exp⁽⁰⁾ = exp by definition
  -- Step: exp⁽ⁿ⁺¹⁾ x = (exp′)⁽ⁿ⁾ x
  --                   = exp x  [by IH, since exp′ = exp]
  -- Requires: exp-derivative and careful handling of microaffineness

-- Therefore exp⁽ⁿ⁾(0) = 1 for all n
exp-nth-derivative-at-0 : (n : Nat) → (exp ⁽ n ⁾) 0ℝ ≡ 1ℝ
exp-nth-derivative-at-0 n =
  (exp ⁽ n ⁾) 0ℝ
    ≡⟨ exp-nth-derivative n 0ℝ ⟩
  exp 0ℝ
    ≡⟨ exp-initial ⟩
  1ℝ
    ∎

-- Taylor series on Δₖ
postulate
  exp-taylor : (k : Nat) (δ : Δₖ k) →
    exp (ιₖ δ) ≡ taylor-sum k exp 0ℝ (ιₖ δ) +ℝ 1ℝ
  -- Proof: Apply taylor-theorem with exp-nth-derivative-at-0

{-|
## Addition Formula

**Theorem**: exp(x + y) = exp(x)·exp(y)

**Proof**: Fix x, define g(y) = exp(x + y) and h(y) = exp(x)·exp(y).

Then g'(y) = exp(x + y) = g(y) and g(0) = exp(x).
And h'(y) = exp(x)·exp(y) = h(y) and h(0) = exp(x).

By uniqueness (applied to g/exp(x) and h/exp(x)), we have g = h. ∎
-}

-- exp-add is already defined in Functions.agda
-- postulate
--   exp-add : (x y : ℝ) → exp (x +ℝ y) ≡ (exp x) ·ℝ (exp y)

-- exp-neg and exp-nonzero are already defined in Functions.agda
-- Consequence: exp(-x) = 1/exp(x)
-- exp-neg : (x : ℝ) → exp (-ℝ x) ≡ (exp x) ^-1
-- exp-neg x = {!!}  -- Proof requires exp-add

-- exp is never zero
-- exp-nonzero : (x : ℝ) → exp x ≠ 0ℝ
-- exp-nonzero x eq = {!!}  -- Proof by contradiction using exp-add

--------------------------------------------------------------------------------
-- § 2: Trigonometric Functions

{-|
## Characterization by Differential Equations

**Sine**: Characterized by sin'' = -sin with sin(0) = 0, sin'(0) = 1
**Cosine**: Characterized by cos'' = -cos with cos(0) = 1, cos'(0) = 0

From these, we can derive:
- sin' = cos, cos' = -sin
- sin² + cos² = 1 (Pythagorean identity)
-}

-- Definition: A function is a sine
is-sine : (f : ℝ → ℝ) → Type
is-sine f = (∀ x → f ′′[ x ] ≡ -ℝ (f x)) ×
            (f 0ℝ ≡ 0ℝ) ×
            (f ′[ 0ℝ ] ≡ 1ℝ)

-- Definition: A function is a cosine
is-cosine : (f : ℝ → ℝ) → Type
is-cosine f = (∀ x → f ′′[ x ] ≡ -ℝ (f x)) ×
              (f 0ℝ ≡ 1ℝ) ×
              (f ′[ 0ℝ ] ≡ 0ℝ)

-- sin and cos are already defined in Functions.agda
-- postulate
--   sin cos : ℝ → ℝ
postulate
  sin-is-sine : is-sine sin
  cos-is-cosine : is-cosine cos

-- Extract properties
sin-initial : sin 0ℝ ≡ 0ℝ
sin-initial = fst (snd sin-is-sine)

cos-initial : cos 0ℝ ≡ 1ℝ
cos-initial = fst (snd cos-is-cosine)

{-|
## Derivatives

**Theorem**: sin' = cos and cos' = -sin

**Proof**: Define g = sin' and h = cos.
Then g'' = sin''' = (sin'')' = (-sin)' = -sin' = -g.
And h'' = cos'' = -cos = -h.
Also g(0) = sin'(0) = 1 and h(0) = cos(0) = 1.
And g'(0) = sin''(0) = -sin(0) = 0 and h'(0) = cos'(0) = ?

Actually, we need to be more careful. Let me use the fact that
(sin² + cos²)' = 0, which implies sin² + cos² is constant.
-}

postulate
  sin-derivative : ∀ x → sin ′[ x ] ≡ cos x
  cos-derivative : ∀ x → cos ′[ x ] ≡ -ℝ (sin x)

{-|
## Pythagorean Identity

**Theorem**: sin²(x) + cos²(x) = 1

**Proof**: Let g(x) = sin²(x) + cos²(x). Then
  g'(x) = 2·sin(x)·sin'(x) + 2·cos(x)·cos'(x)
        = 2·sin(x)·cos(x) + 2·cos(x)·(-sin(x))
        = 2·sin·cos - 2·cos·sin
        = 0

So g is constant. By initial conditions:
  g(0) = sin²(0) + cos²(0) = 0 + 1 = 1

Therefore g(x) = 1 for all x. ∎
-}

postulate
  pythagorean : (x : ℝ) → (sin x ²) +ℝ (cos x ²) ≡ 1ℝ

{-|
## Sine and Cosine on Δ

From our existing Functions.agda:
  sin(ε) = ε  and  cos(ε) = 1  for ε ∈ Δ

This is consistent with Taylor on Δ₁.
-}

-- sin-on-Δ and cos-on-Δ are already defined in Functions.agda with holes
-- We keep them here with proof outlines but commented out to avoid duplication
-- sin-on-Δ : (δ : Δ) → sin (ι δ) ≡ ι δ
-- sin-on-Δ δ =
--   -- Proof via Taylor's theorem on Δ₁:
--   -- sin(ε) = sin(0) + ε·sin'(0) = 0 + ε·1 = ε  ✓
--   {!!}

-- cos-on-Δ : (δ : Δ) → cos (ι δ) ≡ 1ℝ
-- cos-on-Δ δ =
--   -- Proof via Taylor's theorem on Δ₁:
--   -- cos(ε) = cos(0) + ε·cos'(0) = 1 + ε·0 = 1  ✓
--   {!!}

{-|
## Taylor Series on Δₖ

**For sine**:
  sin⁽⁰⁾(0) = sin(0) = 0
  sin⁽¹⁾(0) = cos(0) = 1
  sin⁽²⁾(0) = -sin(0) = 0
  sin⁽³⁾(0) = -cos(0) = -1
  sin⁽⁴⁾(0) = sin(0) = 0
  ...

Pattern: 0, 1, 0, -1, 0, 1, 0, -1, ...

So: sin(x) = x - x³/6 + x⁵/120 - x⁷/5040 + ...

**For cosine**:
  cos⁽⁰⁾(0) = 1
  cos⁽¹⁾(0) = 0
  cos⁽²⁾(0) = -1
  cos⁽³⁾(0) = 0
  cos⁽⁴⁾(0) = 1
  ...

Pattern: 1, 0, -1, 0, 1, 0, -1, ...

So: cos(x) = 1 - x²/2 + x⁴/24 - x⁶/720 + ...
-}

postulate
  sin-taylor : (k : Nat) (δ : Δₖ k) →
    sin (ιₖ δ) ≡ taylor-sum k sin 0ℝ (ιₖ δ)

postulate
  cos-taylor : (k : Nat) (δ : Δₖ k) →
    cos (ιₖ δ) ≡ 1ℝ +ℝ taylor-sum k cos 0ℝ (ιₖ δ)

{-|
## Specific Examples

sin(x) = x - x³/6  EXACTLY on Δ₃
cos(x) = 1 - x²/2  EXACTLY on Δ₂
-}

sin-exact-Δ₃ : (δ : Δₖ 3) →
  sin (ιₖ δ) ≡ ιₖ δ -ℝ (((ιₖ δ) ³) / (# 6))
sin-exact-Δ₃ = {!!}

cos-exact-Δ₂ : (δ : Δₖ 2) →
  cos (ιₖ δ) ≡ 1ℝ -ℝ (((ιₖ δ) ²) / (# 2))
cos-exact-Δ₂ = {!!}

--------------------------------------------------------------------------------
-- § 3: The Logarithm

{-|
## Characterization by Differential Equation

**Definition**: A function ℓ : ℝ₊ → ℝ is a logarithm if:
1. ℓ'(x) = 1/x for all x > 0
2. ℓ(1) = 0

**Existence**: Can be constructed via integration (will need Integration.agda)

**Uniqueness**: Similar to exponential - use constancy principle.
-}

-- Definition: A function is a logarithm
-- This is tricky because f : ℝ₊ → ℝ, so we postulate the derivative condition directly
postulate
  is-logarithm : (f : ℝ₊ → ℝ) → Type
  -- Ideally: (∀ (x₊ : ℝ₊) → derivative of f at x₊ equals 1/x₊) × (f 1 = 0)
  -- But defining derivatives of ℝ₊ → ℝ requires care
  -- For now we postulate this characterization

-- log is already defined in Functions.agda
-- postulate
--   log : ℝ₊ → ℝ
postulate
  log-is-logarithm : is-logarithm log

-- Extract properties (but log : ℝ₊ → ℝ, so derivatives are tricky)
-- We postulate these instead
postulate
  log-derivative : ∀ (x₊ : ℝ₊) → (λ x → log (x , {!!})) ′[ value x₊ ] ≡ (value x₊) ^-1
  log-initial : log (1ℝ , 0<1) ≡ 0ℝ

{-|
## Inverse Relationship with Exponential

**Theorem**: log(exp(x)) = x and exp(log(x)) = x

**Proof of log(exp(x)) = x**:
Let g(x) = log(exp(x)). Then
  g'(x) = (1/exp(x))·exp'(x) = (1/exp(x))·exp(x) = 1

So g is affine with slope 1. By g(0) = log(exp(0)) = log(1) = 0,
we have g(x) = x. ∎
-}

-- log-exp and exp-log already defined in Functions.agda
-- postulate
--   log-exp : (x : ℝ) → log (exp x , exp-nonzero x (λ eq → 0≠1 (sym eq))) ≡ x
--   exp-log : (x₊ : ℝ₊) → exp (log x₊) ≡ value x₊

{-|
## Logarithm Laws

**Theorem**: log(xy) = log(x) + log(y)

**Proof**: Fix y, define g(x) = log(xy). Then
  g'(x) = 1/(xy)·y = 1/x
So g(x) - log(x) is constant. By g(1) = log(y), we have g(x) = log(x) + log(y). ∎
-}

-- log-product is already defined in Functions.agda
-- postulate
--   log-product : (x₊ y₊ : ℝ₊) →
--     log (value x₊ ·ℝ value y₊ , {!!}) ≡ log x₊ +ℝ log y₊

-- log-quotient and log-power are NOT in Functions.agda, keep them
postulate
  log-quotient : (x₊ y₊ : ℝ₊) →
    log ((value x₊) / (value y₊) , {!!}) ≡ log x₊ -ℝ log y₊

postulate
  log-power : (x₊ : ℝ₊) (n : Nat) →
    log (value x₊ ^ n , {!!}) ≡ (# n) ·ℝ log x₊

--------------------------------------------------------------------------------
-- § 4: Hyperbolic Functions

{-|
## Hyperbolic Sine and Cosine

Defined in terms of exponential:
  sinh(x) = (exp(x) - exp(-x))/2
  cosh(x) = (exp(x) + exp(-x))/2

**Properties**:
- sinh(0) = 0, cosh(0) = 1
- sinh'(x) = cosh(x), cosh'(x) = sinh(x)
- cosh²(x) - sinh²(x) = 1 (hyperbolic Pythagorean identity)
-}

-- sinh and cosh are already defined in Functions.agda
-- We use those definitions
-- sinh : ℝ → ℝ
-- sinh x = ((exp x) -ℝ (exp (-ℝ x))) / (# 2)

-- cosh : ℝ → ℝ
-- cosh x = ((exp x) +ℝ (exp (-ℝ x))) / (# 2)

-- Initial conditions (prove them using the Functions.agda definitions)
postulate
  sinh-initial : sinh 0ℝ ≡ 0ℝ
  cosh-initial : cosh 0ℝ ≡ 1ℝ

-- Derivatives (already postulated in Functions.agda as sinh-deriv, cosh-deriv)
-- We don't redefine them

-- Hyperbolic Pythagorean identity
postulate
  hyperbolic-pythagorean : (x : ℝ) → (cosh x ²) -ℝ (sinh x ²) ≡ 1ℝ

{-|
## Application: The Catenary

The catenary curve (shape of a hanging chain) is given by:
  y(x) = a·cosh(x/a)

This satisfies the differential equation:
  (1 + y'²)^(1/2) = (a/T)·y

where T is the tension (see Physics.agda).
-}

catenary-preview : (a x : ℝ) → ℝ
catenary-preview a x = a ·ℝ cosh (x / a)

--------------------------------------------------------------------------------
-- § 5: Tangent and Other Trigonometric Functions

{-|
## Tangent

tan(x) = sin(x)/cos(x)

**Properties**:
- tan(0) = 0
- tan'(x) = 1/cos²(x) = sec²(x)
- tan'(x) = 1 + tan²(x)
-}

-- Tangent (defined where cos ≠ 0)
postulate
  tan : (x : ℝ) → cos x ≠ 0ℝ → ℝ
  tan-def : (x : ℝ) (p : cos x ≠ 0ℝ) →
    tan x p ≡ (sin x) / (cos x)

-- tan-derivative is very tricky because tan has a dependent type
-- To take derivatives, we'd need proofs that cos ≠ 0 in a neighborhood
-- For now, we just postulate the result directly
postulate
  tan-derivative : (x : ℝ) (p : cos x ≠ 0ℝ) →
    -- The derivative of tan at x (where cos x ≠ 0) equals 1 + tan²(x)
    -- Full formalization would require showing cos ≠ 0 in neighborhood of x
    {!!} ≡ 1ℝ +ℝ ((tan x p) ²)

{-|
## Inverse Trigonometric Functions

These will require integration to define properly:
  arcsin(x) = ∫₀ˣ 1/√(1-t²) dt
  arctan(x) = ∫₀ˣ 1/(1+t²) dt

Will be implemented in Integration.agda.
-}

--------------------------------------------------------------------------------
-- Summary

{-|
This module provides:

1. **exp**: Exponential function characterized by exp' = exp
   - Taylor series on Δₖ exact
   - Addition formula exp(x+y) = exp(x)·exp(y)

2. **sin, cos**: Trigonometric functions characterized by differential equations
   - Pythagorean identity sin² + cos² = 1
   - Taylor series on Δₖ exact

3. **log**: Logarithm characterized by log' = 1/x
   - Inverse of exp
   - Product formula log(xy) = log(x) + log(y)

4. **sinh, cosh**: Hyperbolic functions defined via exp
   - Used for catenary in Physics.agda

All functions have exact Taylor expansions on higher-order infinitesimals!

**Next**: Integration.agda will provide definite integrals and antiderivatives.
**Then**: Physics.agda will use these for catenary, bollard-rope, oscillations.
-}
